coq/Examples/Otway_rees.v
@@ -10,87 +10,90 @@ Open Scope string.
 Definition init: proc :=
   mkProc
   [(0, Chan); (1, Name); (2, Name); (3, Skey)]
-  (
+  [
    (* Send (otway_rees.scm:12:6) *)
-   Bind (4, Text) (Nonce) (
-   Bind (5, Mesg) (Pair 2 4) (
-   Bind (6, Mesg) (Pair 1 5) (
-   Send 0 6 (
+   Bind (4, Text) (Nonce);
+   Bind (5, Mesg) (Pair 2 4);
+   Bind (6, Mesg) (Pair 1 5);
+   Send 0 6;
    (* Recv (otway_rees.scm:13:6) *)
-   Bind (7, Mesg) (Recv 0) (
-   Bind (8, Mesg) (Decr 7 3) (
-   Bind (9, Text) (Frst 8) (
-   Bind (10, Mesg) (Scnd 8) (
-   Same 9 4 (
-   Bind (11, Name) (Frst 10) (
-   Bind (12, Mesg) (Scnd 10) (
-   Same 11 1 (
-   Bind (13, Name) (Frst 12) (
-   Bind (14, Skey) (Scnd 12) (
-   Same 13 2 (
-   Return [14])))))))))))))))).
+   Bind (7, Mesg) (Recv 0);
+   Bind (8, Mesg) (Decr 7 3);
+   Bind (9, Text) (Frst 8);
+   Bind (10, Mesg) (Scnd 8);
+   Same 9 4;
+   Bind (11, Name) (Frst 10);
+   Bind (12, Mesg) (Scnd 10);
+   Same 11 1;
+   Bind (13, Name) (Frst 12);
+   Bind (14, Skey) (Scnd 12);
+   Same 13 2;
+   Return [14]
+  ].
 
 (** Role: resp (otway_rees.scm:20:3) *)
 
 Definition resp: proc :=
   mkProc
   [(0, Chan); (1, Chan); (2, Name); (3, Skey)]
-  (
+  [
    (* Recv (otway_rees.scm:24:6) *)
-   Bind (4, Mesg) (Recv 0) (
-   Bind (5, Name) (Frst 4) (
-   Bind (6, Mesg) (Scnd 4) (
-   Bind (7, Name) (Frst 6) (
-   Bind (8, Text) (Scnd 6) (
-   Same 7 2 (
+   Bind (4, Mesg) (Recv 0);
+   Bind (5, Name) (Frst 4);
+   Bind (6, Mesg) (Scnd 4);
+   Bind (7, Name) (Frst 6);
+   Bind (8, Text) (Scnd 6);
+   Same 7 2;
    (* Send (otway_rees.scm:25:6) *)
-   Bind (9, Text) (Nonce) (
-   Bind (10, Mesg) (Pair 8 9) (
-   Bind (11, Mesg) (Pair 2 10) (
-   Bind (12, Mesg) (Pair 5 11) (
-   Send 1 12 (
+   Bind (9, Text) (Nonce);
+   Bind (10, Mesg) (Pair 8 9);
+   Bind (11, Mesg) (Pair 2 10);
+   Bind (12, Mesg) (Pair 5 11);
+   Send 1 12;
    (* Recv (otway_rees.scm:26:6) *)
-   Bind (13, Mesg) (Recv 1) (
-   Bind (14, Mesg) (Frst 13) (
-   Bind (15, Mesg) (Scnd 13) (
-   Bind (16, Mesg) (Decr 15 3) (
-   Bind (17, Text) (Frst 16) (
-   Bind (18, Mesg) (Scnd 16) (
-   Same 17 9 (
-   Bind (19, Name) (Frst 18) (
-   Bind (20, Mesg) (Scnd 18) (
-   Same 19 5 (
-   Bind (21, Name) (Frst 20) (
-   Bind (22, Skey) (Scnd 20) (
-   Same 21 2 (
+   Bind (13, Mesg) (Recv 1);
+   Bind (14, Mesg) (Frst 13);
+   Bind (15, Mesg) (Scnd 13);
+   Bind (16, Mesg) (Decr 15 3);
+   Bind (17, Text) (Frst 16);
+   Bind (18, Mesg) (Scnd 16);
+   Same 17 9;
+   Bind (19, Name) (Frst 18);
+   Bind (20, Mesg) (Scnd 18);
+   Same 19 5;
+   Bind (21, Name) (Frst 20);
+   Bind (22, Skey) (Scnd 20);
+   Same 21 2;
    (* Send (otway_rees.scm:27:6) *)
-   Send 0 14 (
-   Return [5; 22])))))))))))))))))))))))))).
+   Send 0 14;
+   Return [5; 22]
+  ].
 
 (** Role: serv (otway_rees.scm:34:3) *)
 
 Definition serv: proc :=
   mkProc
   [(0, Chan); (1, Name); (2, Name); (3, Skey); (4, Skey)]
-  (
+  [
    (* Recv (otway_rees.scm:37:6) *)
-   Bind (5, Mesg) (Recv 0) (
-   Bind (6, Name) (Frst 5) (
-   Bind (7, Mesg) (Scnd 5) (
-   Same 6 1 (
-   Bind (8, Name) (Frst 7) (
-   Bind (9, Mesg) (Scnd 7) (
-   Same 8 2 (
-   Bind (10, Text) (Frst 9) (
-   Bind (11, Text) (Scnd 9) (
+   Bind (5, Mesg) (Recv 0);
+   Bind (6, Name) (Frst 5);
+   Bind (7, Mesg) (Scnd 5);
+   Same 6 1;
+   Bind (8, Name) (Frst 7);
+   Bind (9, Mesg) (Scnd 7);
+   Same 8 2;
+   Bind (10, Text) (Frst 9);
+   Bind (11, Text) (Scnd 9);
    (* Send (otway_rees.scm:38:6) *)
-   Bind (12, Skey) (Nonce) (
-   Bind (13, Mesg) (Pair 2 12) (
-   Bind (14, Mesg) (Pair 1 13) (
-   Bind (15, Mesg) (Pair 10 14) (
-   Bind (16, Mesg) (Encr 15 3) (
-   Bind (17, Mesg) (Pair 11 14) (
-   Bind (18, Mesg) (Encr 17 4) (
-   Bind (19, Mesg) (Pair 16 18) (
-   Send 0 19 (
-   Return [12]))))))))))))))))))).
+   Bind (12, Skey) (Nonce);
+   Bind (13, Mesg) (Pair 2 12);
+   Bind (14, Mesg) (Pair 1 13);
+   Bind (15, Mesg) (Pair 10 14);
+   Bind (16, Mesg) (Encr 15 3);
+   Bind (17, Mesg) (Pair 11 14);
+   Bind (18, Mesg) (Encr 17 4);
+   Bind (19, Mesg) (Pair 16 18);
+   Send 0 19;
+   Return [12]
+  ].
