coq/Examples/Yahalom.v
@@ -10,91 +10,95 @@ Open Scope string.
 Definition init: proc :=
   mkProc
   [(0, Chan); (1, Chan); (2, Name); (3, Name); (4, Skey)]
-  (
+  [
    (* Send (yahalom.scm:13:6) *)
-   Bind (5, Text) (Nonce) (
-   Bind (6, Mesg) (Pair 2 5) (
-   Send 0 6 (
+   Bind (5, Text) (Nonce);
+   Bind (6, Mesg) (Pair 2 5);
+   Send 0 6;
    (* Recv (yahalom.scm:14:6) *)
-   Bind (7, Mesg) (Recv 1) (
-   Bind (8, Mesg) (Frst 7) (
-   Bind (9, Mesg) (Scnd 7) (
-   Bind (10, Mesg) (Decr 8 4) (
-   Bind (11, Name) (Frst 10) (
-   Bind (12, Mesg) (Scnd 10) (
-   Same 11 3 (
-   Bind (13, Skey) (Frst 12) (
-   Bind (14, Mesg) (Scnd 12) (
-   Bind (15, Text) (Frst 14) (
-   Bind (16, Text) (Scnd 14) (
-   Same 15 5 (
+   Bind (7, Mesg) (Recv 1);
+   Bind (8, Mesg) (Frst 7);
+   Bind (9, Mesg) (Scnd 7);
+   Bind (10, Mesg) (Decr 8 4);
+   Bind (11, Name) (Frst 10);
+   Bind (12, Mesg) (Scnd 10);
+   Same 11 3;
+   Bind (13, Skey) (Frst 12);
+   Bind (14, Mesg) (Scnd 12);
+   Bind (15, Text) (Frst 14);
+   Bind (16, Text) (Scnd 14);
+   Same 15 5;
    (* Send (yahalom.scm:15:6) *)
-   Bind (17, Mesg) (Encr 16 13) (
-   Bind (18, Mesg) (Pair 9 17) (
-   Send 0 18 (
-   Return [13]))))))))))))))))))).
+   Bind (17, Mesg) (Encr 16 13);
+   Bind (18, Mesg) (Pair 9 17);
+   Send 0 18;
+   Return [13]
+  ].
 
 (** Role: resp (yahalom.scm:23:3) *)
 
 Definition resp: proc :=
   mkProc
   [(0, Chan); (1, Chan); (2, Name); (3, Skey)]
-  (
+  [
    (* Recv (yahalom.scm:26:6) *)
-   Bind (4, Mesg) (Recv 0) (
-   Bind (5, Name) (Frst 4) (
-   Bind (6, Text) (Scnd 4) (
+   Bind (4, Mesg) (Recv 0);
+   Bind (5, Name) (Frst 4);
+   Bind (6, Text) (Scnd 4);
    (* Send (yahalom.scm:27:6) *)
-   Bind (7, Text) (Nonce) (
-   Bind (8, Mesg) (Pair 6 7) (
-   Bind (9, Mesg) (Pair 5 8) (
-   Bind (10, Mesg) (Encr 9 3) (
-   Bind (11, Mesg) (Pair 2 10) (
-   Send 1 11 (
+   Bind (7, Text) (Nonce);
+   Bind (8, Mesg) (Pair 6 7);
+   Bind (9, Mesg) (Pair 5 8);
+   Bind (10, Mesg) (Encr 9 3);
+   Bind (11, Mesg) (Pair 2 10);
+   Send 1 11;
    (* Recv (yahalom.scm:28:6) *)
-   Bind (12, Mesg) (Recv 0) (
-   Bind (13, Mesg) (Frst 12) (
-   Bind (14, Mesg) (Scnd 12) (
-   Bind (15, Mesg) (Decr 13 3) (
-   Bind (16, Name) (Frst 15) (
-   Bind (17, Skey) (Scnd 15) (
-   Same 16 5 (
-   Bind (18, Text) (Decr 14 17) (
-   Same 18 7 (
-   Return [5; 17]))))))))))))))))))).
+   Bind (12, Mesg) (Recv 0);
+   Bind (13, Mesg) (Frst 12);
+   Bind (14, Mesg) (Scnd 12);
+   Bind (15, Mesg) (Decr 13 3);
+   Bind (16, Name) (Frst 15);
+   Bind (17, Skey) (Scnd 15);
+   Same 16 5;
+   Bind (18, Text) (Decr 14 17);
+   Same 18 7;
+   Return [5; 17]
+  ].
 
 (** Role: serv-init (yahalom.scm:36:3) *)
 
 Definition serv_init: proc :=
   mkProc
   [(0, Chan); (1, Name); (2, Skey)]
-  (
+  [
    (* Recv (yahalom.scm:39:6) *)
-   Bind (3, Mesg) (Recv 0) (
-   Bind (4, Name) (Frst 3) (
-   Bind (5, Mesg) (Scnd 3) (
-   Same 4 1 (
-   Bind (6, Mesg) (Decr 5 2) (
-   Bind (7, Name) (Frst 6) (
-   Bind (8, Mesg) (Scnd 6) (
-   Bind (9, Text) (Frst 8) (
-   Bind (10, Text) (Scnd 8) (
-   Return [7; 9; 10])))))))))).
+   Bind (3, Mesg) (Recv 0);
+   Bind (4, Name) (Frst 3);
+   Bind (5, Mesg) (Scnd 3);
+   Same 4 1;
+   Bind (6, Mesg) (Decr 5 2);
+   Bind (7, Name) (Frst 6);
+   Bind (8, Mesg) (Scnd 6);
+   Bind (9, Text) (Frst 8);
+   Bind (10, Text) (Scnd 8);
+   Return [7; 9; 10]
+  ].
 
 (** Role: serv-complete (yahalom.scm:45:3) *)
 
 Definition serv_complete: proc :=
   mkProc
   [(0, Chan); (1, Name); (2, Name); (3, Skey); (4, Skey); (5, Text); (6, Text)]
-  (
+  [
    (* Send (yahalom.scm:48:6) *)
-   Bind (7, Skey) (Nonce) (
-   Bind (8, Mesg) (Pair 5 6) (
-   Bind (9, Mesg) (Pair 7 8) (
-   Bind (10, Mesg) (Pair 2 9) (
-   Bind (11, Mesg) (Encr 10 3) (
-   Bind (12, Mesg) (Pair 1 7) (
-   Bind (13, Mesg) (Encr 12 4) (
-   Bind (14, Mesg) (Pair 11 13) (
-   Send 0 14 (
-   Return [7])))))))))).
+   Bind (7, Skey) (Nonce);
+   Bind (8, Mesg) (Pair 5 6);
+   Bind (9, Mesg) (Pair 7 8);
+   Bind (10, Mesg) (Pair 2 9);
+   Bind (11, Mesg) (Encr 10 3);
+   Bind (12, Mesg) (Pair 1 7);
+   Bind (13, Mesg) (Encr 12 4);
+   Bind (14, Mesg) (Pair 11 13);
+   Send 0 14;
+   Return [7]
+  ].
