coq/SemTactics.v
@@ -48,7 +48,8 @@ Ltac sem_inv :=
     | [ H: lookup _ _ = _ |- _ ] => inv H
     | [ H: sort_check _ _ |- _ ] => inv H
     | [ H: expr_sem _ _ _ _ _ _ _ _ |- _ ] => inv H
-    | [ H: stmts_sem _ _ _ _ _ _ |- _ ] => inv H
+    | [ H: stmt_sem _ _ _ _ _ _ _ |- _ ] => inv H
+    | [ H: stmt_list_sem _ _ _ _ _ _ _ _ |- _ ] => inv H
     end.
 
 Ltac sem_rewrite :=
