coq/Unilateral.v
@@ -10,25 +10,27 @@ Open Scope string.
 Definition init: proc :=
   mkProc
   [(0, Chan); (1, Akey)]
-  (
+  [
    (* Send (../rtst/unilateral.scm:9:7) *)
-   Bind (2, Text) (Nonce) (
-   Bind (3, Mesg) (Encr 2 1) (
-   Send 0 3 (
+   Bind (2, Text) (Nonce);
+   Bind (3, Mesg) (Encr 2 1);
+   Send 0 3;
    (* Recv (../rtst/unilateral.scm:10:7) *)
-   Bind (4, Text) (Recv 0) (
-   Same 4 2 (
-   Return [2])))))).
+   Bind (4, Text) (Recv 0);
+   Same 4 2;
+   Return [2]
+  ].
 
 (** Role: resp (../rtst/unilateral.scm:14:3) *)
 
 Definition resp: proc :=
   mkProc
   [(0, Chan); (1, Ikey)]
-  (
+  [
    (* Recv (../rtst/unilateral.scm:17:7) *)
-   Bind (2, Mesg) (Recv 0) (
-   Bind (3, Text) (Decr 2 1) (
+   Bind (2, Mesg) (Recv 0);
+   Bind (3, Text) (Decr 2 1);
    (* Send (../rtst/unilateral.scm:18:7) *)
-   Send 0 3 (
-   Return [3])))).
+   Send 0 3;
+   Return [3]
+  ].
