coq/Unilateral_proof.v
@@ -76,14 +76,15 @@ Qed.
 Definition bad_init: proc :=
   mkProc
   [(0, Chan); (1, Akey)]
-  (
+  [
    (* Send (rtst/unilateral.scm:9:7) *)
-   Bind (2, Text) (Nonce) (
-   Bind (3, Mesg) (Encr 2 1) (
-   Send 0 3 (
+   Bind (2, Text) (Nonce);
+   Bind (3, Mesg) (Encr 2 1);
+   Send 0 3;
    (* Recv (rtst/unilateral.scm:10:7) *)
-   Bind (4, Text) (Recv 0) (
-   Return [2]))))).
+   Bind (4, Text) (Recv 0);
+   Return [2]
+  ].
 
 (** Liveness is okay. *)
 
